rpc/impl.v
@@ -25,34 +25,34 @@ Definition listen : val := λ: "c", Conn.listen "c".
 Definition confirm : val := λ: "c" "skB" "req",
   Conn.confirm "c" "skB" "req".
 
-Definition call : val := λ: "c" "cs" "N" "ts",
-  Conn.write "c" "cs" "N" "ts";;
-  Conn.read "c" "cs" (Tag $ rpcN.@"resp").
+Definition call : val := λ: "cs" "N" "ts",
+  Conn.write "cs" "N" "ts";;
+  Conn.read "cs" (Tag $ rpcN.@"resp").
 
-Definition handle : val := λ: "c" "N" "f",
+Definition handle : val := λ: "N" "f",
   Conn.handle "N"
     (λ: "cs" "ts",
       match: "f" "ts" with
-        SOME "res" => Conn.write "c" "cs" (Tag (rpcN.@"resp")) "res"
-      | NONE => Conn.write "c" "cs" (Tag (rpcN.@"error")) [TInt 0]
+        SOME "res" => Conn.write "cs" (Tag (rpcN.@"resp")) "res"
+      | NONE => Conn.write "cs" (Tag (rpcN.@"error")) [TInt 0]
       end;;
       #true).
 
-Definition close : val := λ: "c" "cs",
-  Conn.write "c" "cs" (Tag $ rpcN.@"close") [TInt 0];;
-  Conn.read  "c" "cs" (Tag $ rpcN.@"resp");;
-  Conn.free "c" "cs".
+Definition close : val := λ: "cs",
+  Conn.write "cs" (Tag $ rpcN.@"close") [TInt 0];;
+  Conn.read  "cs" (Tag $ rpcN.@"resp");;
+  Conn.free "cs".
 
-Definition handle_close : val := λ: "c",
+Definition handle_close : expr :=
   Conn.handle (Tag $ rpcN.@"close")
     (λ: "cs" "ts",
-      Conn.write "c" "cs" (Tag (rpcN.@"resp")) [TInt 0];;
-      Conn.free "c" "cs";;
-      #false).
+      Conn.write "cs" (Tag (rpcN.@"resp")) [TInt 0];;
+      Conn.free "cs";;
+      #false)%V.
 
-Definition server : val := rec: "loop" "c" "cs" "handlers" :=
-  let: "cont" := Conn.select "c" "cs" (handle_close "c" :: "handlers") in
-  if: "cont" then "loop" "c" "cs" "handlers"
+Definition server : val := rec: "loop" "cs" "handlers" :=
+  let: "cont" := Conn.select "cs" (handle_close :: "handlers") in
+  if: "cont" then "loop" "cs" "handlers"
   else #().
 
 End Impl.
