store/client_proofs/store.v
@@ -25,17 +25,16 @@ Implicit Types n : nat.
 Implicit Types γ : gname.
 Implicit Types v : val.
 
-Lemma wp_client_store c kI kR cs t1 t2 t2' :
-  channel c -∗
+Lemma wp_client_store kI kR cs t1 t2 t2' :
   cryptis_ctx -∗
   store_ctx -∗
   public t1 -∗
   public t2' -∗
   {{{ db_connected kI kR cs ∗ db_mapsto kI kR t1 t2 }}}
-    Client.store c (repr cs) t1 t2'
+    Client.store (repr cs) t1 t2'
   {{{ RET #(); db_connected kI kR cs ∗ db_mapsto kI kR t1 t2' }}}.
 Proof.
-iIntros "#chan_c #? #ctx #p_t1 #p_t2 !> %Φ [client mapsto] post".
+iIntros "#? #ctx #p_t1 #p_t2 !> %Φ [client mapsto] post".
 iDestruct "client" as "(conn & db)".
 iMod (store_call t2' with "db mapsto") as "(store & mapsto & waiting)".
 wp_lam. wp_pures. wp_list.
